start replacing lists with vectors and get basic implementation working

Validator/Expr/IfExpr.lean
@@ -1,3 +1,6 @@
+import Mathlib.Data.Vector.Snoc
+import Mathlib.Data.Vector.MapLemmas
+
 import Validator.Expr.Pred
 import Validator.Expr.Regex
 import Validator.Expr.Grammar
@@ -5,7 +8,7 @@ import Validator.Expr.Grammar
 inductive IfExpr μ α where
   | mk (cnd: Pred α) (thn: Fin μ)
 
-abbrev IfExprs μ α := List (IfExpr μ α)
+abbrev IfExprs μ α ν := List.Vector (IfExpr μ α) ν
 
 namespace IfExpr
 
@@ -16,15 +19,10 @@ def eval {α: Type} [DecidableEq α] (g: Grammar μ α Pred) (ifExpr: IfExpr μ 
     then g.lookup thn
     else Regex.emptyset
 
-def evals {α: Type} {μ: Nat} [DecidableEq α] (g: Grammar μ α Pred) (ifExprs: IfExprs μ α) (t: α): List (Rule μ α Pred) :=
-  List.map (fun x => eval g x t) ifExprs
+def evals {α: Type} {μ: Nat} [DecidableEq α] (g: Grammar μ α Pred) (ifExprs: IfExprs μ α ν) (t: α): Rules μ α Pred ν :=
+  List.Vector.map (fun x => eval g x t) ifExprs
 
 theorem evals_nil_is_nil {α: Type} {μ: Nat} [DecidableEq α] (g: Grammar μ α Pred) (a: α):
-  evals g (μ := μ) [] a = [] := by
-  unfold evals
-  simp
-
-theorem evals_concat_is_concat {α: Type} [DecidableEq α] (g: Grammar μ α Pred) (xs ys: IfExprs μ α) (a: α):
-  evals g (xs ++ ys) a = evals g xs a ++ evals g ys a := by
+  evals g (μ := μ) List.Vector.nil a = List.Vector.nil := by
   unfold evals
   simp
