Validator/Derive/Enter.lean
@@ -1,33 +1,19 @@
+import Mathlib.Data.Vector.Snoc
+
 import Validator.Expr.Regex
 import Validator.Expr.Grammar
 import Validator.Expr.IfExpr
+import Validator.Expr.Symbol
 
 namespace Enter
 
-def enter (x: Rule μ α Pred) (res: IfExprs μ α := []): IfExprs μ α :=
-  match x with
-  | Regex.emptyset => res
-  | Regex.emptystr => res
-  | Regex.symbol (pred, childRef) => (IfExpr.mk pred childRef) :: res
-  | Regex.or y z => enter y (enter z res)
-  | Regex.concat y z =>
-    if Regex.nullable y
-    then enter y (enter z res)
-    else enter y res
-  | Regex.star y => enter y res
-
-def deriveEnter (xs: Rules μ α Pred): IfExprs μ α :=
-  List.flatten (List.map Enter.enter xs)
-
-theorem deriveEnter_nil_is_nil {α: Type} {μ: Nat}:
-  @deriveEnter μ α [] = [] := by
-  unfold deriveEnter
-  simp
-
-theorem deriveEnter_cons_is_concat {α: Type} (x: Rule μ α Pred) (xs: Rules μ α Pred):
-  deriveEnter (x::xs) = (deriveEnter [x]) ++ (deriveEnter xs) := by
-  unfold deriveEnter
-  simp
+def deriveEnter (xs: Rules μ α Pred ν): IfExprs μ α (Symbol.nums xs) :=
+  List.Vector.map
+    (fun (pred, ref) => IfExpr.mk pred ref)
+    (Symbol.Symbols.cast
+      (Symbol.extracts xs List.Vector.nil).2
+      (by ac_rfl)
+    )
 
 class DeriveEnter (m: Type -> Type u) (μ: Nat) (α: outParam Type)  where
-  deriveEnter (xs: Rules μ α Pred): m (IfExprs μ α)
+  deriveEnter (xs: Rules μ α Pred ν): m (IfExprs μ α (Symbol.nums xs))
