Validator/Expr/Compress.lean
@@ -7,7 +7,7 @@ inductive Index where
  | val (n: Nat)
  | emptyset -- emptyset is unescapable, so it gets a special index
 
-def indexOf [DecidableEq α] (xs: Rules μ α Pred) (y: (Rule μ α Pred)): Except String Index :=
+def indexOf [DecidableEq α] (xs: List (Regex (Pred α × Ref μ))) (y: (Rule μ α Pred)): Except String Index :=
   match y with
   | Regex.emptyset => Except.ok Index.emptyset
   | _ =>
@@ -15,15 +15,15 @@ def indexOf [DecidableEq α] (xs: Rules μ α Pred) (y: (Rule μ α Pred)): Exce
     | Option.none => Except.error "indexOf: unable to find expression"
     | Option.some idx => Except.ok (Index.val idx)
 
-def ofIndex' (xs: Rules μ α Pred) (index: Nat): Except String (Rule μ α Pred) :=
+def ofIndex' (xs: Rules μ α Pred ν) (index: Nat): Except String (Rule μ α Pred) :=
   match xs with
-  | [] => Except.error "index overflow"
-  | (x::xs') =>
+  | ⟨[], _⟩ => Except.error "index overflow"
+  | ⟨x::xs', h⟩ =>
     match index with
     | 0 => Except.ok x
-    | (n' + 1) => ofIndex' xs' n'
+    | (n' + 1) => ofIndex' ⟨xs', congrArg Nat.pred h⟩ n'
 
-def ofIndex (xs: Rules μ α Pred) (index: Index): Except String (Rule μ α Pred) :=
+def ofIndex (xs: Rules μ α Pred ν) (index: Index): Except String (Rule μ α Pred) :=
   match index with
   | Index.emptyset => Except.ok Regex.emptyset
   | Index.val n =>
@@ -35,26 +35,45 @@ def ofIndex (xs: Rules μ α Pred) (index: Index): Except String (Rule μ α Pre
 inductive Indices where
   | mk (indices: List Index)
 
+def compressed [DecidableEq α] (xs: Rules μ α Pred ν): Nat :=
+  (List.erase (List.eraseReps xs.toList) Regex.emptyset).length
+
 -- compress compresses a list of expressions.
-def compress [DecidableEq α] (xs: Rules μ α Pred): Except String ((Rules μ α Pred) × Indices) := do
+def compress [DecidableEq α] (xs: Rules μ α Pred ν1): Except String ((Rules μ α Pred (compressed xs)) × Indices) := do
   -- sort to increase chance of cache hit
   -- TODO: let sxs := List.mergeSort xs
   -- remove duplicates
-  let sxs' := List.eraseReps xs
+  let sxs' := List.eraseReps xs.toList
   -- remove unescapable expressions, currently only emptyset
-  let sxs'': Rules μ α Pred := List.erase sxs' Regex.emptyset
+  let sxs'' := List.erase sxs' Regex.emptyset
   -- find all indexes of the original expressions in the compressed expressions
-  let indexes: List Index <- List.mapM (indexOf sxs'') xs
-  return (sxs'', Indices.mk indexes)
+  let indexes: List Index <- List.mapM (indexOf sxs'') xs.toList
+  return (
+    Subtype.mk
+      sxs'' (by
+        simp only [sxs'', sxs']
+        rfl
+      ),
+    Indices.mk indexes
+  )
 
-def compressM [DecidableEq α] [Monad m] [MonadExcept String m] (xs: Rules μ α Pred): m ((Rules μ α Pred) × Indices) := do
+def compressM [DecidableEq α] [Monad m] [MonadExcept String m] (xs: Rules μ α Pred ν1): m ((Rules μ α Pred (compressed xs)) × Indices) := do
   MonadExcept.ofExcept (compress xs)
 
 -- expand expands a list of expressions.
-def expand (indices: Indices) (xs: Rules μ α Pred): Except String (Rules μ α Pred) :=
+def expand (indices: Indices) (xs: Rules μ α Pred ν1): Except String ((ν2: Nat) × (Rules μ α Pred ν2)) :=
   match indices with
   | Indices.mk indexes =>
-    List.mapM (ofIndex xs) indexes
+    match MonadExcept.ofExcept (List.mapM (ofIndex xs) indexes) with
+    | Except.error e => Except.error e
+    | Except.ok k => Except.ok (
+      Sigma.mk
+        k.length
+        (Subtype.mk
+          k
+          rfl
+        )
+      )
 
-def expandM [Monad m] [MonadExcept String m] (indices: Indices) (xs: Rules μ α Pred): m (Rules μ α Pred) :=
+def expandM [Monad m] [MonadExcept String m] (indices: Indices) (xs: Rules μ α Pred ν1): m ((ν2: Nat) × (Rules μ α Pred ν2)) :=
   MonadExcept.ofExcept (expand indices xs)
